<?xml version="1.0"?>
<rdf:RDF xmlns="http://scientificvariablesontology.org#"
     xml:base="http://scientificvariablesontology.org"
     xmlns:opla="http://ontologydesignpatterns.org/opla#"
     xmlns:rdf="http://www.w3.org/1999/02/22-rdf-syntax-ns#"
     xmlns:owl="http://www.w3.org/2002/07/owl#"
     xmlns:xml="http://www.w3.org/XML/1998/namespace"
     xmlns:xsd="http://www.w3.org/2001/XMLSchema#"
     xmlns:rdfs="http://www.w3.org/2000/01/rdf-schema#">
    <owl:Ontology rdf:about="http://scientificvariablesontology.org">
        <owl:versionIRI rdf:resource="http://scientificvariablesontology.org/2.0.0"/>
        <rdfs:comment>Scientific Variables Ontology ver 2.0.0</rdfs:comment>
    </owl:Ontology>
    


    <!-- 
    ///////////////////////////////////////////////////////////////////////////////////////
    //
    // Classes
    //
    ///////////////////////////////////////////////////////////////////////////////////////
     -->

    


    <!-- http://scientificvariablesontology.org#Abstraction -->

    <owl:Class rdf:about="http://scientificvariablesontology.org#Abstraction">
        <rdfs:comment>a complementary entity to a Phenomenon, Property, or Phenomenon building block, that is a mathematical representation of that entity</rdfs:comment>
    </owl:Class>
    


    <!-- http://scientificvariablesontology.org#Attribute -->

    <owl:Class rdf:about="http://scientificvariablesontology.org#Attribute">
        <rdfs:comment>an ontological construct that provides a generic design pattern for attaching a property and associated value to a phenomenon to specify one of its set characteristics from the perspective of an identified scientific variable</rdfs:comment>
    </owl:Class>
    


    <!-- http://scientificvariablesontology.org#Context -->

    <owl:Class rdf:about="http://scientificvariablesontology.org#Context">
        <rdfs:comment>an ontological construct that creates a link between two phenomena to indicate that one phenomenon provides spatiotemporal information for the other phenomenon, from the perspective of the focus phenomena of an identified scientific variable</rdfs:comment>
    </owl:Class>
    


    <!-- http://scientificvariablesontology.org#Form -->

    <owl:Class rdf:about="http://scientificvariablesontology.org#Form">
        <rdfs:subClassOf rdf:resource="http://scientificvariablesontology.org#Attribute"/>
    </owl:Class>
    


    <!-- http://scientificvariablesontology.org#Matter -->

    <owl:Class rdf:about="http://scientificvariablesontology.org#Matter">
        <rdfs:subClassOf rdf:resource="http://scientificvariablesontology.org#Attribute"/>
    </owl:Class>
    


    <!-- http://scientificvariablesontology.org#Part -->

    <owl:Class rdf:about="http://scientificvariablesontology.org#Part">
        <rdfs:subClassOf rdf:resource="http://scientificvariablesontology.org#Attribute"/>
    </owl:Class>
    


    <!-- http://scientificvariablesontology.org#Participant -->

    <owl:Class rdf:about="http://scientificvariablesontology.org#Participant">
        <rdfs:comment>an ontological construct that links a Phenomenon participating in a Phenomenon with a Process and assigns that Phenomenon a role in the Process</rdfs:comment>
    </owl:Class>
    


    <!-- http://scientificvariablesontology.org#ParticipantRole -->

    <owl:Class rdf:about="http://scientificvariablesontology.org#ParticipantRole">
        <rdfs:comment>a reification that identifies a Phenomenon&apos;s function in another Phenomenon that involves a Process</rdfs:comment>
    </owl:Class>
    


    <!-- http://scientificvariablesontology.org#Phenomenon -->

    <owl:Class rdf:about="http://scientificvariablesontology.org#Phenomenon">
        <rdfs:comment>anything (concrete) that can be or is observed to exist or happen in the physical universe</rdfs:comment>
    </owl:Class>
    


    <!-- http://scientificvariablesontology.org#Process -->

    <owl:Class rdf:about="http://scientificvariablesontology.org#Process">
        <rdfs:comment>an act or activity in which a phenomenon participates that changes the state of that phenomenon. Processes may involve multiple participants.</rdfs:comment>
    </owl:Class>
    


    <!-- http://scientificvariablesontology.org#Property -->

    <owl:Class rdf:about="http://scientificvariablesontology.org#Property">
        <rdfs:comment>any characteristic or quality of a Phenomenon or Abstraction</rdfs:comment>
    </owl:Class>
    


    <!-- http://scientificvariablesontology.org#PropertyRole -->

    <owl:Class rdf:about="http://scientificvariablesontology.org#PropertyRole">
        <rdfs:comment>the part assumed by a Variable in an Abstraction</rdfs:comment>
    </owl:Class>
    


    <!-- http://scientificvariablesontology.org#Reference -->

    <owl:Class rdf:about="http://scientificvariablesontology.org#Reference">
        <rdfs:comment>an ontological construct that creates a link between two variables to indicate that the value of one variable provides a reference for the assessment of the value of the second variable</rdfs:comment>
    </owl:Class>
    


    <!-- http://scientificvariablesontology.org#Role -->

    <owl:Class rdf:about="http://scientificvariablesontology.org#Role">
        <rdfs:subClassOf rdf:resource="http://scientificvariablesontology.org#Attribute"/>
    </owl:Class>
    


    <!-- http://scientificvariablesontology.org#ScientificVariable -->

    <owl:Class rdf:about="http://scientificvariablesontology.org#ScientificVariable">
        <rdfs:comment>an identifier for a Property-Phenomenon pairing that idicates a unique physical system and/or abstraction of a physical system and corresponding characteristic being observed or modeled by a scientist</rdfs:comment>
    </owl:Class>
    


    <!-- http://scientificvariablesontology.org#SpatiotemporalRelationship -->

    <owl:Class rdf:about="http://scientificvariablesontology.org#SpatiotemporalRelationship">
        <rdfs:comment>reification that identifies the connection between two Phenomena or Variables</rdfs:comment>
    </owl:Class>
    


    <!-- http://scientificvariablesontology.org#VariableRole -->

    <owl:Class rdf:about="http://scientificvariablesontology.org#VariableRole">
        <rdfs:comment>the function or part assument by a Phenomenon in a Variable</rdfs:comment>
    </owl:Class>
</rdf:RDF>



<!-- Generated by the OWL API (version 4.2.8.20170104-2310) https://github.com/owlcs/owlapi -->

